Refactor code based on new nested ind. tree def

ExistentialRules/Terms/Basic.lean
@@ -20,27 +20,10 @@ abbrev PreGroundTerm (sig : Signature) [DecidableEq sig.C] [DecidableEq sig.V] :
 
 namespace PreGroundTerm
 
-  mutual
-
-    def arity_ok {sig : Signature} [DecidableEq sig.C] [DecidableEq sig.V] : FiniteTree (SkolemFS sig) sig.C -> Bool
-    | .leaf _ => true
-    | .inner func ts =>
-      ts.toList.length == func.arity && arity_ok_list ts
-
-    def arity_ok_list {sig : Signature} [DecidableEq sig.C] [DecidableEq sig.V] : FiniteTreeList (SkolemFS sig) sig.C -> Bool
-    | .nil => true
-    | .cons hd tl => arity_ok hd && arity_ok_list tl
-
-  end
-
-  theorem arity_ok_list_iff_arity_ok_each_mem {sig : Signature} [DecidableEq sig.C] [DecidableEq sig.V] (ts : FiniteTreeList (SkolemFS sig) sig.C) : (∀ t, t ∈ ts.toList -> PreGroundTerm.arity_ok t) ↔ PreGroundTerm.arity_ok_list ts := by
-    cases ts with
-    | nil => simp [arity_ok_list, FiniteTreeList.toList]
-    | cons hd tl =>
-      unfold arity_ok_list
-      simp [FiniteTreeList.toList]
-      intro _
-      apply arity_ok_list_iff_arity_ok_each_mem
+  def arity_ok {sig : Signature} [DecidableEq sig.C] [DecidableEq sig.V] : FiniteTree (SkolemFS sig) sig.C -> Bool
+  | .leaf _ => true
+  | .inner func ts =>
+    ts.length == func.arity && ts.attach.all (fun ⟨t, _⟩ => arity_ok t)
 
 end PreGroundTerm
 
@@ -62,23 +45,20 @@ variable {sig : Signature} [DecidableEq sig.C] [DecidableEq sig.V]
 namespace GroundTerm
 
   def const (c : sig.C) : GroundTerm sig := ⟨FiniteTree.leaf c, by simp [PreGroundTerm.arity_ok]⟩
-  def func (func : SkolemFS sig) (ts : List (GroundTerm sig)) (arity_ok : ts.length = func.arity) : GroundTerm sig := ⟨FiniteTree.inner func (FiniteTreeList.fromList ts.unattach), by
+  def func (func : SkolemFS sig) (ts : List (GroundTerm sig)) (arity_ok : ts.length = func.arity) : GroundTerm sig := ⟨FiniteTree.inner func ts.unattach, by
     unfold PreGroundTerm.arity_ok
     rw [Bool.and_eq_true, beq_iff_eq]
-    rw [FiniteTreeList.fromListToListIsId]
     constructor
     . rw [List.length_unattach]; exact arity_ok
-    . rw [← PreGroundTerm.arity_ok_list_iff_arity_ok_each_mem]
-      rw [FiniteTreeList.fromListToListIsId]
+    . rw [List.all_eq_true]
       intro t t_mem
       unfold List.unattach at t_mem
-      rw [List.mem_map] at t_mem
+      rw [List.attach_map, List.mem_map] at t_mem
       rcases t_mem with ⟨t, t_mem, t_eq⟩
       rw [← t_eq]
-      exact t.property
+      exact t.val.property
   ⟩
 
-  -- TODO: we are barely using cases and rec for GroundTerm; use it more or remove it if it turns out to not be useful
   @[elab_as_elim, cases_eliminator]
   def cases
       {motive : GroundTerm sig -> Sort u}
@@ -91,14 +71,14 @@ namespace GroundTerm
       have eq : t = GroundTerm.const c := Subtype.eq eq
       eq ▸ const c
     | .inner f ts => by
-      let ts : List (GroundTerm sig) := ts.toList.attach.map (fun ⟨t', mem⟩ => ⟨t', by
+      let ts : List (GroundTerm sig) := ts.attach.map (fun ⟨t', mem⟩ => ⟨t', by
         have prop := t.property
         unfold PreGroundTerm.arity_ok at prop
         simp only [eq, Bool.and_eq_true, beq_iff_eq] at prop
         have prop := prop.right
-        rw [← PreGroundTerm.arity_ok_list_iff_arity_ok_each_mem] at prop
-        apply prop
-        exact mem
+        rw [List.all_eq_true] at prop
+        apply prop ⟨t', mem⟩
+        apply List.mem_attach
       ⟩)
       have arity_ok : ts.length = f.arity := by
         have prop := t.property
@@ -113,7 +93,7 @@ namespace GroundTerm
         simp [eq, ts]
         unfold List.unattach
         rw [List.map_map, List.map_attach_eq_pmap]
-        simp [FiniteTreeList.toListFromListIsId]
+        simp
       exact eq ▸ (func f ts arity_ok)
 
   @[elab_as_elim, induction_eliminator]
@@ -128,14 +108,14 @@ namespace GroundTerm
       have eq : t = GroundTerm.const c := Subtype.eq eq_val
       eq ▸ const c
     | .inner f ts => by
-      let ts : List (GroundTerm sig) := ts.toList.attach.map (fun ⟨t', mem⟩ => ⟨t', by
+      let ts : List (GroundTerm sig) := ts.attach.map (fun ⟨t', mem⟩ => ⟨t', by
         have prop := t.property
         unfold PreGroundTerm.arity_ok at prop
         simp only [eq_val, Bool.and_eq_true, beq_iff_eq] at prop
         have prop := prop.right
-        rw [← PreGroundTerm.arity_ok_list_iff_arity_ok_each_mem] at prop
-        apply prop
-        exact mem
+        rw [List.all_eq_true] at prop
+        apply prop ⟨t', mem⟩
+        apply List.mem_attach
       ⟩)
       have arity_ok : ts.length = f.arity := by
         have prop := t.property
@@ -150,7 +130,7 @@ namespace GroundTerm
         simp [eq_val, ts]
         unfold List.unattach
         rw [List.map_map, List.map_attach_eq_pmap]
-        simp [FiniteTreeList.toListFromListIsId]
+        simp
       exact eq ▸ (func f ts arity_ok (by
         intro t' mem
         have : t'.val.depth < t.val.depth := by
@@ -158,8 +138,8 @@ namespace GroundTerm
           simp only [eq_val]
           rw [Nat.add_comm]
           apply Nat.lt_add_one_of_le
-          apply FiniteTree.depth_le_depthList_of_mem
-          unfold ts at mem
+          apply List.le_max?_getD_of_mem
+          apply List.mem_map_of_mem
           rw [List.mem_map] at mem
           rcases mem with ⟨s, s_mem, t_eq⟩
           simp at t_eq
@@ -193,27 +173,7 @@ namespace GroundTerm
   theorem depth_func (f : SkolemFS sig) (ts : List (GroundTerm sig)) (arity_ok : ts.length = f.arity) :
       (GroundTerm.func f ts arity_ok).depth = 1 + (((ts.map (GroundTerm.depth)).max?).getD 1) := by
     simp only [GroundTerm.func, depth, FiniteTree.depth]
-
-    have : ∀ (ts : List (GroundTerm sig)), (FiniteTree.depthList (FiniteTreeList.fromList ts.unattach)) = (((ts.map (GroundTerm.depth)).max?).getD 1) := by
-      intro ts
-      induction ts with
-      | nil => simp [FiniteTreeList.fromList, FiniteTree.depthList]
-      | cons hd tl ih =>
-        rw [List.map_cons, List.max?_cons, List.unattach_cons]
-        unfold FiniteTree.depthList
-        unfold FiniteTreeList.fromList
-        simp only [Option.getD_some]
-        cases eq : (tl.map depth).max? with
-        | some m => simp only [Option.elim]; rw [ih, eq, Option.getD_some]; rfl
-        | none =>
-          simp only [Option.elim]
-          rw [List.max?_eq_none_iff, List.map_eq_nil_iff] at eq
-          rw [eq]
-          simp only [FiniteTreeList.fromList, FiniteTree.depthList, List.unattach_nil]
-          rw [Nat.max_eq_left]
-          . rfl
-          . unfold FiniteTree.depth; cases hd.val <;> simp
-
+    have : ts.map depth = ts.unattach.map FiniteTree.depth := by rw [List.map_unattach]; rfl
     rw [this]
 
   theorem constants_const (c : sig.C) : (GroundTerm.const c).constants = [c] := by
@@ -222,20 +182,8 @@ namespace GroundTerm
   theorem constants_func (f : SkolemFS sig) (ts : List (GroundTerm sig)) (arity_ok : ts.length = f.arity) :
       (GroundTerm.func f ts arity_ok).constants = ts.flatMap GroundTerm.constants := by
     simp only [GroundTerm.func, constants, FiniteTree.leaves]
-
-    have : ∀ (ts : List (GroundTerm sig)), (FiniteTree.leavesList (FiniteTreeList.fromList ts.unattach)) = (ts.flatMap GroundTerm.constants) := by
-      intro ts
-      induction ts with
-      | nil => simp [FiniteTreeList.fromList, FiniteTree.leavesList]
-      | cons hd tl ih =>
-        rw [List.flatMap_cons, List.unattach_cons]
-        unfold FiniteTree.leavesList
-        unfold FiniteTreeList.fromList
-        simp only
-        rw [ih]
-        rfl
-
-    rw [this]
+    rw [List.flatMap_unattach]
+    rfl
 
   theorem functions_const (c : sig.C) : (GroundTerm.const c).functions = [] := by
     simp [GroundTerm.const, functions, FiniteTree.innerLabels]
@@ -243,20 +191,11 @@ namespace GroundTerm
   theorem functions_func (f : SkolemFS sig) (ts : List (GroundTerm sig)) (arity_ok : ts.length = f.arity) :
       (GroundTerm.func f ts arity_ok).functions = f :: (ts.flatMap GroundTerm.functions) := by
     simp only [GroundTerm.func, functions, FiniteTree.innerLabels]
-
-    have : ∀ (ts : List (GroundTerm sig)), (FiniteTree.innerLabelsList (FiniteTreeList.fromList ts.unattach)) = (ts.flatMap GroundTerm.functions) := by
-      intro ts
-      induction ts with
-      | nil => simp [FiniteTreeList.fromList, FiniteTree.innerLabelsList]
-      | cons hd tl ih =>
-        rw [List.flatMap_cons, List.unattach_cons]
-        unfold FiniteTree.innerLabelsList
-        unfold FiniteTreeList.fromList
-        simp only
-        rw [ih]
-        rfl
-
-    rw [this]
+    rw [List.cons_eq_cons]
+    constructor
+    . rfl
+    . rw [List.flatMap_unattach]
+      rfl
 
 end GroundTerm
 
