ExistentialRules/ChaseSequence/Termination/BacktrackingOfFacts/PreTrigger.lean
@@ -1,0 +1,328 @@
+import ExistentialRules.ChaseSequence.Termination.BacktrackingOfFacts.GroundTerm
+
+variable {sig : Signature} [DecidableEq sig.P] [DecidableEq sig.C] [DecidableEq sig.V]
+
+namespace PreTrigger
+
+  def skolem_ruleIds_valid (rl : RuleList sig) (trg : PreTrigger sig) : Prop := ∀ t ∈ trg.mapped_body.flatMap GeneralizedAtom.terms, t.skolem_ruleIds_valid rl
+  def skolem_disjIdx_valid (rl : RuleList sig) (trg : PreTrigger sig) (trg_ruleIds_valid : trg.skolem_ruleIds_valid rl) : Prop :=
+    ∀ t, (h : t ∈ trg.mapped_body.flatMap GeneralizedAtom.terms) -> t.skolem_disjIdx_valid rl (trg_ruleIds_valid t h)
+  def skolem_rule_arity_valid (rl : RuleList sig) (trg : PreTrigger sig) (trg_ruleIds_valid : trg.skolem_ruleIds_valid rl) : Prop :=
+    ∀ t, (h : t ∈ trg.mapped_body.flatMap GeneralizedAtom.terms) -> t.skolem_rule_arity_valid rl (trg_ruleIds_valid t h)
+
+  theorem skolem_ruleIds_valid_of_strong_equiv {rl : RuleList sig} {trg trg2 : PreTrigger sig} (strong_equiv : trg.strong_equiv trg2) (trg_valid : trg.skolem_ruleIds_valid rl) : trg2.skolem_ruleIds_valid rl := by
+    unfold skolem_ruleIds_valid; rw [← PreTrigger.mapped_body_eq_of_strong_equiv strong_equiv]; exact trg_valid
+
+  theorem skolem_disjIdx_valid_of_strong_equiv {rl : RuleList sig} {trg trg2 : PreTrigger sig} (strong_equiv : trg.strong_equiv trg2) (h : trg.skolem_ruleIds_valid rl) (trg_valid : trg.skolem_disjIdx_valid rl h) : trg2.skolem_disjIdx_valid rl (PreTrigger.skolem_ruleIds_valid_of_strong_equiv strong_equiv h) := by
+    unfold skolem_disjIdx_valid; simp only [← PreTrigger.mapped_body_eq_of_strong_equiv strong_equiv]; exact trg_valid
+
+  theorem skolem_rule_arity_valid_of_strong_equiv {rl : RuleList sig} {trg trg2 : PreTrigger sig} (strong_equiv : trg.strong_equiv trg2) (h : trg.skolem_ruleIds_valid rl) (trg_valid : trg.skolem_rule_arity_valid rl h) : trg2.skolem_rule_arity_valid rl (PreTrigger.skolem_ruleIds_valid_of_strong_equiv strong_equiv h) := by
+    unfold skolem_rule_arity_valid; simp only [← PreTrigger.mapped_body_eq_of_strong_equiv strong_equiv]; exact trg_valid
+
+  theorem skolem_ruleIds_valid_for_functional_term
+      (rl : RuleList sig)
+      (trg : PreTrigger sig)
+      (rule_mem : trg.rule ∈ rl.rules)
+      (body_valid : trg.skolem_ruleIds_valid rl) :
+      ∀ i v, (trg.functional_term_for_var i v).skolem_ruleIds_valid rl := by
+    intro i v
+    simp only [GroundTerm.skolem_ruleIds_valid, PreGroundTerm.skolem_ruleIds_valid, PreTrigger.functional_term_for_var, GroundTerm.func]
+    constructor
+    . exists trg.rule
+    . intro t t_mem
+      rw [List.mem_unattach] at t_mem
+      rcases t_mem with ⟨h, t_mem⟩
+      rw [List.mem_map] at t_mem
+      rcases t_mem with ⟨v, v_mem, t_eq⟩
+      apply body_valid ⟨t, h⟩
+      rcases trg.rule.frontier_occurs_in_body v v_mem with ⟨a, a_mem, hd_mem⟩
+      rw [List.mem_flatMap]
+      exists trg.subs.apply_function_free_atom a
+      constructor
+      . apply List.mem_map_of_mem; exact a_mem
+      . unfold GroundSubstitution.apply_function_free_atom
+        unfold TermMapping.apply_generalized_atom
+        rw [List.mem_map]
+        exists VarOrConst.var v
+
+  theorem skolem_disjIdx_valid_for_functional_term
+      (rl : RuleList sig)
+      (trg : PreTrigger sig)
+      (rule_mem : trg.rule ∈ rl.rules)
+      (trg_ruleIds_valid : trg.skolem_ruleIds_valid rl)
+      (body_valid : trg.skolem_disjIdx_valid rl trg_ruleIds_valid) :
+      ∀ i v, (i < trg.rule.head.length) -> (trg.functional_term_for_var i v).skolem_disjIdx_valid rl (trg.skolem_ruleIds_valid_for_functional_term rl rule_mem trg_ruleIds_valid i v) := by
+    intro i v i_lt
+    simp only [GroundTerm.skolem_disjIdx_valid, PreGroundTerm.skolem_disjIdx_valid, GroundTerm.func, functional_term_for_var]
+    constructor
+    . unfold SkolemFS.disjunctIndex_valid
+      rw [rl.get_by_id_self _ rule_mem]
+      exact i_lt
+    . have func_ruleIds_valid := trg.skolem_ruleIds_valid_for_functional_term rl rule_mem trg_ruleIds_valid i v
+      intro t t_mem
+      rw [List.mem_unattach] at t_mem
+      rcases t_mem with ⟨h, t_mem⟩
+      rw [List.mem_map] at t_mem
+      rcases t_mem with ⟨v, v_mem, t_eq⟩
+      apply body_valid ⟨t, h⟩
+      rcases trg.rule.frontier_occurs_in_body v v_mem with ⟨a, a_mem, hd_mem⟩
+      rw [List.mem_flatMap]
+      exists trg.subs.apply_function_free_atom a
+      constructor
+      . apply List.mem_map_of_mem; exact a_mem
+      . unfold GroundSubstitution.apply_function_free_atom
+        unfold TermMapping.apply_generalized_atom
+        rw [List.mem_map]
+        exists VarOrConst.var v
+
+  theorem skolem_rule_arity_valid_for_functional_term
+      (rl : RuleList sig)
+      (trg : PreTrigger sig)
+      (rule_mem : trg.rule ∈ rl.rules)
+      (trg_ruleIds_valid : trg.skolem_ruleIds_valid rl)
+      (body_valid : trg.skolem_rule_arity_valid rl trg_ruleIds_valid) :
+      ∀ i v, (trg.functional_term_for_var i v).skolem_rule_arity_valid rl (trg.skolem_ruleIds_valid_for_functional_term rl rule_mem trg_ruleIds_valid i v) := by
+    intro i v
+    simp only [GroundTerm.skolem_rule_arity_valid, PreGroundTerm.skolem_rule_arity_valid, GroundTerm.func, functional_term_for_var]
+    constructor
+    . unfold SkolemFS.arity_valid
+      rw [rl.get_by_id_self _ rule_mem]
+    . have func_ruleIds_valid := trg.skolem_ruleIds_valid_for_functional_term rl rule_mem trg_ruleIds_valid i v
+      intro t t_mem
+      rw [List.mem_unattach] at t_mem
+      rcases t_mem with ⟨h, t_mem⟩
+      rw [List.mem_map] at t_mem
+      rcases t_mem with ⟨v, v_mem, t_eq⟩
+      apply body_valid ⟨t, h⟩
+      rcases trg.rule.frontier_occurs_in_body v v_mem with ⟨a, a_mem, hd_mem⟩
+      rw [List.mem_flatMap]
+      exists trg.subs.apply_function_free_atom a
+      constructor
+      . apply List.mem_map_of_mem; exact a_mem
+      . unfold GroundSubstitution.apply_function_free_atom
+        unfold TermMapping.apply_generalized_atom
+        rw [List.mem_map]
+        exists VarOrConst.var v
+
+  theorem skolem_ruleIds_remain_valid_in_head (rl : RuleList sig) (trg : PreTrigger sig) (rule_mem : trg.rule ∈ rl.rules) (body_valid : trg.skolem_ruleIds_valid rl) :
+      ∀ t ∈ trg.mapped_head.flatten.flatMap GeneralizedAtom.terms, t.skolem_ruleIds_valid rl := by
+    intro t t_mem
+    rw [List.mem_flatMap] at t_mem
+    rcases t_mem with ⟨f, f_mem, t_mem⟩
+    rw [List.mem_flatten] at f_mem
+    rcases f_mem with ⟨l, l_mem, f_mem⟩
+    let disj_idx : Fin trg.mapped_head.length := ⟨trg.mapped_head.idxOf l, by apply List.idxOf_lt_length_of_mem; exact l_mem⟩
+    let voc : VarOrConst sig := trg.var_or_const_for_result_term disj_idx (by rw [List.getElem_idxOf_of_mem l_mem]; exact f_mem) t_mem
+    rw [← trg.apply_on_var_or_const_for_result_term_is_term disj_idx (by rw [List.getElem_idxOf_of_mem l_mem]; exact f_mem) t_mem]
+    cases eq : voc with
+    | const c =>
+      unfold voc at eq
+      rw [eq, trg.apply_to_var_or_const_for_const disj_idx.val _]
+      apply GroundTerm.skolem_ruleIds_valid_const
+    | var v =>
+      cases Decidable.em (v ∈ trg.rule.frontier) with
+      | inl mem_frontier =>
+        unfold voc at eq
+        rw [eq, trg.apply_to_var_or_const_frontier_var disj_idx.val _ mem_frontier]
+        apply body_valid
+        rcases trg.rule.frontier_occurs_in_body v mem_frontier with ⟨a, a_mem, v_mem⟩
+        rw [List.mem_flatMap]
+        exists trg.subs.apply_function_free_atom a
+        constructor
+        . apply List.mem_map_of_mem; exact a_mem
+        . unfold GroundSubstitution.apply_function_free_atom
+          unfold TermMapping.apply_generalized_atom
+          rw [List.mem_map]
+          exists VarOrConst.var v
+      | inr mem_frontier =>
+        unfold voc at eq
+        rw [eq, trg.apply_to_var_or_const_non_frontier_var disj_idx.val _ mem_frontier]
+        apply skolem_ruleIds_valid_for_functional_term
+        . exact rule_mem
+        . exact body_valid
+
+  theorem skolem_disjIdx_remains_valid_in_head
+      (rl : RuleList sig)
+      (trg : PreTrigger sig)
+      (rule_mem : trg.rule ∈ rl.rules)
+      (trg_ruleIds_valid : trg.skolem_ruleIds_valid rl)
+      (body_valid : trg.skolem_disjIdx_valid rl trg_ruleIds_valid) :
+      ∀ t, (t_mem : t ∈ trg.mapped_head.flatten.flatMap GeneralizedAtom.terms) -> t.skolem_disjIdx_valid rl (trg.skolem_ruleIds_remain_valid_in_head rl rule_mem trg_ruleIds_valid t t_mem) := by
+    intro t t_mem
+    rw [List.mem_flatMap] at t_mem
+    rcases t_mem with ⟨f, f_mem, t_mem⟩
+    rw [List.mem_flatten] at f_mem
+    rcases f_mem with ⟨l, l_mem, f_mem⟩
+    let disj_idx : Fin trg.mapped_head.length := ⟨trg.mapped_head.idxOf l, by apply List.idxOf_lt_length_of_mem; exact l_mem⟩
+
+    cases t with
+    | const c => apply GroundTerm.skolem_disjIdx_valid_const
+    | func fs ts arity_ok =>
+      cases Decidable.em ((GroundTerm.func fs ts arity_ok) ∈ trg.rule.frontier.map trg.subs) with
+      | inl t_mem_frontier =>
+        rw [List.mem_map] at t_mem_frontier
+        rcases t_mem_frontier with ⟨v, v_mem, v_eq⟩
+        apply body_valid
+        rcases trg.rule.frontier_occurs_in_body v v_mem with ⟨a, a_mem, v_mem⟩
+        rw [List.mem_flatMap]
+        exists trg.subs.apply_function_free_atom a
+        constructor
+        . apply List.mem_map_of_mem; exact a_mem
+        . unfold GroundSubstitution.apply_function_free_atom
+          unfold TermMapping.apply_generalized_atom
+          rw [List.mem_map]
+          exists VarOrConst.var v
+      | inr t_mem_frontier =>
+        let voc : VarOrConst sig := trg.var_or_const_for_result_term disj_idx (by rw [List.getElem_idxOf_of_mem l_mem]; exact f_mem) t_mem
+        have voc_eq := trg.apply_on_var_or_const_for_result_term_is_term disj_idx (by rw [List.getElem_idxOf_of_mem l_mem]; exact f_mem) t_mem
+        cases eq : voc with
+        | const c =>
+          unfold voc at eq
+          rw [eq, trg.apply_to_var_or_const_for_const disj_idx.val _] at voc_eq
+          simp [GroundTerm.const, GroundTerm.func] at voc_eq
+        | var v =>
+          unfold voc at eq
+          rw [eq] at voc_eq
+          cases Decidable.em (v ∈ trg.rule.frontier) with
+          | inl v_mem_frontier =>
+            rw [trg.apply_to_var_or_const_frontier_var disj_idx.val _ v_mem_frontier] at voc_eq
+            apply False.elim
+            apply t_mem_frontier
+            rw [List.mem_map]
+            exists v
+          | inr v_mem_frontier =>
+            rw [trg.apply_to_var_or_const_non_frontier_var disj_idx.val _ v_mem_frontier] at voc_eq
+            simp only [← voc_eq]
+            apply skolem_disjIdx_valid_for_functional_term
+            . exact rule_mem
+            . exact body_valid
+            . rw [← PreTrigger.length_mapped_head]; exact disj_idx.isLt
+
+  theorem skolem_rule_arity_remains_valid_in_head
+      (rl : RuleList sig)
+      (trg : PreTrigger sig)
+      (rule_mem : trg.rule ∈ rl.rules)
+      (trg_ruleIds_valid : trg.skolem_ruleIds_valid rl)
+      (body_valid : trg.skolem_rule_arity_valid rl trg_ruleIds_valid) :
+      ∀ t, (t_mem : t ∈ trg.mapped_head.flatten.flatMap GeneralizedAtom.terms) -> t.skolem_rule_arity_valid rl (trg.skolem_ruleIds_remain_valid_in_head rl rule_mem trg_ruleIds_valid t t_mem) := by
+    intro t t_mem
+    rw [List.mem_flatMap] at t_mem
+    rcases t_mem with ⟨f, f_mem, t_mem⟩
+    rw [List.mem_flatten] at f_mem
+    rcases f_mem with ⟨l, l_mem, f_mem⟩
+    let disj_idx : Fin trg.mapped_head.length := ⟨trg.mapped_head.idxOf l, by apply List.idxOf_lt_length_of_mem; exact l_mem⟩
+
+    cases t with
+    | const c => apply GroundTerm.skolem_rule_arity_valid_const
+    | func fs ts arity_ok =>
+      cases Decidable.em ((GroundTerm.func fs ts arity_ok) ∈ trg.rule.frontier.map trg.subs) with
+      | inl t_mem_frontier =>
+        rw [List.mem_map] at t_mem_frontier
+        rcases t_mem_frontier with ⟨v, v_mem, v_eq⟩
+        apply body_valid
+        rcases trg.rule.frontier_occurs_in_body v v_mem with ⟨a, a_mem, v_mem⟩
+        rw [List.mem_flatMap]
+        exists trg.subs.apply_function_free_atom a
+        constructor
+        . apply List.mem_map_of_mem; exact a_mem
+        . unfold GroundSubstitution.apply_function_free_atom
+          unfold TermMapping.apply_generalized_atom
+          rw [List.mem_map]
+          exists VarOrConst.var v
+      | inr t_mem_frontier =>
+        let voc : VarOrConst sig := trg.var_or_const_for_result_term disj_idx (by rw [List.getElem_idxOf_of_mem l_mem]; exact f_mem) t_mem
+        have voc_eq := trg.apply_on_var_or_const_for_result_term_is_term disj_idx (by rw [List.getElem_idxOf_of_mem l_mem]; exact f_mem) t_mem
+        cases eq : voc with
+        | const c =>
+          unfold voc at eq
+          rw [eq, trg.apply_to_var_or_const_for_const disj_idx.val _] at voc_eq
+          simp [GroundTerm.const, GroundTerm.func] at voc_eq
+        | var v =>
+          unfold voc at eq
+          rw [eq] at voc_eq
+          cases Decidable.em (v ∈ trg.rule.frontier) with
+          | inl v_mem_frontier =>
+            rw [trg.apply_to_var_or_const_frontier_var disj_idx.val _ v_mem_frontier] at voc_eq
+            apply False.elim
+            apply t_mem_frontier
+            rw [List.mem_map]
+            exists v
+          | inr v_mem_frontier =>
+            rw [trg.apply_to_var_or_const_non_frontier_var disj_idx.val _ v_mem_frontier] at voc_eq
+            simp only [← voc_eq]
+            apply skolem_rule_arity_valid_for_functional_term
+            . exact rule_mem
+            . exact body_valid
+
+  def backtrackTrigger_for_functional_term
+      [GetFreshInhabitant sig.C]
+      [Inhabited sig.C]
+      (rl : RuleList sig)
+      (trg : PreTrigger sig)
+      (trg_rule_mem : trg.rule ∈ rl.rules)
+      (trg_ruleIds_valid : trg.skolem_ruleIds_valid rl)
+      (trg_rule_arity_valid : trg.skolem_rule_arity_valid rl trg_ruleIds_valid)
+      (forbidden_constants : List sig.C)
+      (i : Nat) (v : sig.V) :
+      PreTrigger sig :=
+    ((trg.functional_term_for_var i v).backtrackTrigger rl (by
+      cases eq : trg.functional_term_for_var i v with
+      | const _ => simp [functional_term_for_var, GroundTerm.func, GroundTerm.const] at eq
+      | func func ts arity_ok => exists func, ts, arity_ok
+    ) (by apply trg.skolem_ruleIds_valid_for_functional_term; exact trg_rule_mem; exact trg_ruleIds_valid) (by apply trg.skolem_rule_arity_valid_for_functional_term; exact trg_rule_mem; exact trg_rule_arity_valid) forbidden_constants)
+
+  theorem backtrackTrigger_for_functional_term_equiv
+      [GetFreshInhabitant sig.C]
+      [Inhabited sig.C]
+      (rl : RuleList sig)
+      (trg : PreTrigger sig)
+      (trg_rule_mem : trg.rule ∈ rl.rules)
+      (trg_ruleIds_valid : trg.skolem_ruleIds_valid rl)
+      (trg_rule_arity_valid : trg.skolem_rule_arity_valid rl trg_ruleIds_valid)
+      (forbidden_constants : List sig.C) :
+      ∀ i v, (trg.backtrackTrigger_for_functional_term rl trg_rule_mem trg_ruleIds_valid trg_rule_arity_valid forbidden_constants i v).equiv trg := by
+    intro i v
+    simp only [backtrackTrigger_for_functional_term, PreTrigger.functional_term_for_var, GroundTerm.backtrackTrigger, GroundTerm.func, PreGroundTerm.backtrackTrigger]
+    simp only [PreTrigger.equiv]
+    constructor
+    . apply RuleList.get_by_id_self; exact trg_rule_mem
+    . intro u u_mem
+      simp only [u_mem, ↓reduceDIte]
+      rw [Subtype.mk.injEq]
+      rw [List.getElem_unattach, List.getElem_map]
+      conv => left; right; right; left; rw [RuleList.get_by_id_self _ _ trg_rule_mem]
+      rw [List.getElem_idxOf_of_mem]
+      rw [RuleList.get_by_id_self _ _ trg_rule_mem] at u_mem
+      exact u_mem
+
+  def backtrackFacts
+      [GetFreshInhabitant sig.C]
+      [Inhabited sig.C]
+      (rl : RuleList sig)
+      (trg : PreTrigger sig)
+      (trg_ruleIds_valid : trg.skolem_ruleIds_valid rl)
+      (trg_disjIdx_valid : trg.skolem_disjIdx_valid rl trg_ruleIds_valid)
+      (trg_rule_arity_valid : trg.skolem_rule_arity_valid rl trg_ruleIds_valid) : (List (Fact sig)) × (List sig.C) :=
+    let forbidden_constants := trg.mapped_body.flatMap Fact.constants ++ rl.rules.flatMap Rule.constants
+    let backtrack_result := GroundTerm.backtrackFacts_list rl (trg.mapped_body.flatMap GeneralizedAtom.terms) trg_ruleIds_valid trg_disjIdx_valid trg_rule_arity_valid forbidden_constants
+    (trg.mapped_body ++ backtrack_result.fst, backtrack_result.snd)
+
+  theorem backtrackFacts_eq_of_strong_equiv
+      [GetFreshInhabitant sig.C]
+      [Inhabited sig.C]
+      (rl : RuleList sig)
+      (trg trg2 : PreTrigger sig)
+      (trg_ruleIds_valid : trg.skolem_ruleIds_valid rl)
+      (trg_disjIdx_valid : trg.skolem_disjIdx_valid rl trg_ruleIds_valid)
+      (trg_rule_arity_valid : trg.skolem_rule_arity_valid rl trg_ruleIds_valid)
+      (strong_equiv : trg.strong_equiv trg2) :
+      trg.backtrackFacts rl trg_ruleIds_valid trg_disjIdx_valid trg_rule_arity_valid =
+        trg2.backtrackFacts rl
+          (PreTrigger.skolem_ruleIds_valid_of_strong_equiv strong_equiv trg_ruleIds_valid)
+          (PreTrigger.skolem_disjIdx_valid_of_strong_equiv strong_equiv trg_ruleIds_valid trg_disjIdx_valid)
+          (PreTrigger.skolem_rule_arity_valid_of_strong_equiv strong_equiv trg_ruleIds_valid trg_rule_arity_valid) := by
+    unfold backtrackFacts
+    simp only [PreTrigger.mapped_body_eq_of_strong_equiv strong_equiv]
+
+end PreTrigger
+
