ExistentialRules/ChaseSequence/Termination/RenameConstantsApart/PreTrigger.lean
@@ -1,0 +1,176 @@
+import ExistentialRules.ChaseSequence.Termination.RenameConstantsApart.GroundTerm
+
+variable {sig : Signature} [DecidableEq sig.C] [DecidableEq sig.V]
+
+def GroundSubstitution.rename_constants_apart_for_vars [GetFreshInhabitant sig.C] (subs : GroundSubstitution sig) (forbidden_constants : List sig.C) : List sig.V -> GroundSubstitution sig
+| .nil => subs
+| .cons hd tl =>
+  let renamed_term_for_hd := (subs hd).rename_constants_apart forbidden_constants
+  let new_forbidden := forbidden_constants ++ renamed_term_for_hd.constants
+  fun v => if v = hd then renamed_term_for_hd else
+    subs.rename_constants_apart_for_vars new_forbidden tl v
+
+theorem GroundSubstitution.rename_constants_apart_for_vars_constants_fresh
+    [GetFreshInhabitant sig.C]
+    (subs : GroundSubstitution sig)
+    (forbidden_constants : List sig.C)
+    (vars : List sig.V) :
+    ∀ v ∈ vars, ∀ c ∈ (subs.rename_constants_apart_for_vars forbidden_constants vars v).constants, c ∉ forbidden_constants := by
+  induction vars generalizing forbidden_constants with
+  | nil => intros; contradiction
+  | cons hd tl ih =>
+    intro v v_mem c c_mem
+    cases Decidable.em (v = hd) with
+    | inl v_eq_hd =>
+      simp only [rename_constants_apart_for_vars, v_eq_hd, ↓reduceIte] at c_mem
+      apply GroundTerm.rename_constants_apart_constants_fresh
+      exact c_mem
+    | inr v_neq_hd =>
+      have v_mem : v ∈ tl := by cases v_mem; contradiction; assumption
+      simp only [rename_constants_apart_for_vars, v_neq_hd, ↓reduceIte] at c_mem
+      let new_forbidden := forbidden_constants ++ ((subs hd).rename_constants_apart forbidden_constants).constants
+      specialize ih new_forbidden v v_mem c c_mem
+      intro contra
+      apply ih
+      simp [new_forbidden, contra]
+
+variable [DecidableEq sig.P]
+
+theorem GroundSubstitution.rename_constants_apart_for_vars_preserves_ruleId_validity [GetFreshInhabitant sig.C] (subs : GroundSubstitution sig) (forbidden_constants : List sig.C) (vars : List sig.V) :
+    ∀ rl, ∀ v ∈ vars, (subs v).skolem_ruleIds_valid rl -> (subs.rename_constants_apart_for_vars forbidden_constants vars v).skolem_ruleIds_valid rl := by
+  intro rl v
+  induction vars generalizing forbidden_constants with
+  | nil => intros; contradiction
+  | cons hd tl ih =>
+    intro v_mem
+    rw [List.mem_cons] at v_mem
+    cases Decidable.em (v = hd) with
+    | inl v_eq =>
+      simp only [rename_constants_apart_for_vars, v_eq, ↓reduceIte]
+      apply GroundTerm.rename_constants_apart_preserves_ruleId_validity
+    | inr v_neq =>
+      simp only [rename_constants_apart_for_vars, v_neq, ↓reduceIte]
+      apply ih
+      cases v_mem with
+      | inl v_mem => contradiction
+      | inr v_mem => exact v_mem
+
+theorem GroundSubstitution.rename_constants_apart_for_vars_preserves_disjIdx_validity [GetFreshInhabitant sig.C] (subs : GroundSubstitution sig) (forbidden_constants : List sig.C) (vars : List sig.V) :
+    ∀ rl, ∀ v, (v_mem : v ∈ vars) -> (h : (subs v).skolem_ruleIds_valid rl) -> (subs v).skolem_disjIdx_valid rl h -> (subs.rename_constants_apart_for_vars forbidden_constants vars v).skolem_disjIdx_valid rl (subs.rename_constants_apart_for_vars_preserves_ruleId_validity forbidden_constants vars rl v v_mem h) := by
+  intro rl v
+  induction vars generalizing forbidden_constants with
+  | nil => intros; contradiction
+  | cons hd tl ih =>
+    intro v_mem
+    rw [List.mem_cons] at v_mem
+    cases Decidable.em (v = hd) with
+    | inl v_eq =>
+      simp only [rename_constants_apart_for_vars, v_eq, ↓reduceIte]
+      apply GroundTerm.rename_constants_apart_preserves_disjIdx_validity
+    | inr v_neq =>
+      simp only [rename_constants_apart_for_vars, v_neq, ↓reduceIte]
+      apply ih
+      cases v_mem with
+      | inl v_mem => contradiction
+      | inr v_mem => exact v_mem
+
+theorem GroundSubstitution.rename_constants_apart_for_vars_preserves_rule_arity_validity [GetFreshInhabitant sig.C] (subs : GroundSubstitution sig) (forbidden_constants : List sig.C) (vars : List sig.V) :
+    ∀ rl, ∀ v, (v_mem : v ∈ vars) -> (h : (subs v).skolem_ruleIds_valid rl) -> (subs v).skolem_rule_arity_valid rl h -> (subs.rename_constants_apart_for_vars forbidden_constants vars v).skolem_rule_arity_valid rl (subs.rename_constants_apart_for_vars_preserves_ruleId_validity forbidden_constants vars rl v v_mem h) := by
+  intro rl v
+  induction vars generalizing forbidden_constants with
+  | nil => intros; contradiction
+  | cons hd tl ih =>
+    intro v_mem
+    rw [List.mem_cons] at v_mem
+    cases Decidable.em (v = hd) with
+    | inl v_eq =>
+      simp only [rename_constants_apart_for_vars, v_eq, ↓reduceIte]
+      apply GroundTerm.rename_constants_apart_preserves_rule_arity_validity
+    | inr v_neq =>
+      simp only [rename_constants_apart_for_vars, v_neq, ↓reduceIte]
+      apply ih
+      cases v_mem with
+      | inl v_mem => contradiction
+      | inr v_mem => exact v_mem
+
+
+def PreTrigger.rename_constants_apart [GetFreshInhabitant sig.C] (trg : PreTrigger sig) (forbidden_constants : List sig.C) : PreTrigger sig :=
+  ⟨trg.rule, trg.subs.rename_constants_apart_for_vars forbidden_constants trg.rule.body.vars.eraseDupsKeepRight⟩
+
+theorem PreTrigger.rename_constants_apart_constants_fresh
+    [GetFreshInhabitant sig.C]
+    (trg : PreTrigger sig)
+    (forbidden_constants : List sig.C) :
+    ∀ c ∈ (trg.rule.body.vars.eraseDupsKeepRight.map (trg.rename_constants_apart forbidden_constants).subs).flatMap GroundTerm.constants, c ∉ forbidden_constants := by
+  intro c c_mem
+  rw [List.mem_flatMap] at c_mem
+  rcases c_mem with ⟨t, t_mem, c_mem⟩
+  rw [List.mem_map] at t_mem
+  rcases t_mem with ⟨v, v_mem, t_eq⟩
+  apply trg.subs.rename_constants_apart_for_vars_constants_fresh forbidden_constants trg.rule.body.vars.eraseDupsKeepRight v v_mem
+  rw [← t_eq] at c_mem
+  exact c_mem
+
+theorem PreTrigger.rename_constants_apart_preserves_ruleId_validity [GetFreshInhabitant sig.C] (trg : PreTrigger sig) (forbidden_constants : List sig.C) :
+    ∀ rl, PreTrigger.skolem_ruleIds_valid rl trg -> PreTrigger.skolem_ruleIds_valid rl (PreTrigger.rename_constants_apart trg forbidden_constants) := by
+  intro rl valid
+  unfold skolem_ruleIds_valid at *
+  intro t t_mem
+  rw [mem_terms_mapped_body_iff] at t_mem
+  cases t_mem with
+  | inl t_mem =>
+    rcases t_mem with ⟨c, c_mem, t_eq⟩
+    rw [← t_eq]
+    apply GroundTerm.skolem_ruleIds_valid_const
+  | inr t_mem =>
+    rcases t_mem with ⟨v, v_mem, t_eq⟩
+    rw [← t_eq]
+    apply trg.subs.rename_constants_apart_for_vars_preserves_ruleId_validity forbidden_constants trg.rule.body.vars.eraseDupsKeepRight rl v
+    . rw [List.mem_eraseDupsKeepRight]; exact v_mem
+    . apply valid
+      rw [mem_terms_mapped_body_iff]
+      apply Or.inr
+      exists v
+
+theorem PreTrigger.rename_constants_apart_preserves_disjIdx_validity [GetFreshInhabitant sig.C] (trg : PreTrigger sig) (forbidden_constants : List sig.C) :
+    ∀ rl, (h : PreTrigger.skolem_ruleIds_valid rl trg) -> PreTrigger.skolem_disjIdx_valid rl trg h -> PreTrigger.skolem_disjIdx_valid rl (PreTrigger.rename_constants_apart trg forbidden_constants) (PreTrigger.rename_constants_apart_preserves_ruleId_validity trg forbidden_constants rl h) := by
+  intro rl h valid
+  unfold skolem_disjIdx_valid at *
+  intro t t_mem
+  rw [mem_terms_mapped_body_iff] at t_mem
+  cases t_mem with
+  | inl t_mem =>
+    rcases t_mem with ⟨c, c_mem, t_eq⟩
+    simp only [← t_eq]
+    apply GroundTerm.skolem_disjIdx_valid_const
+  | inr t_mem =>
+    rcases t_mem with ⟨v, v_mem, t_eq⟩
+    simp only [← t_eq]
+    apply trg.subs.rename_constants_apart_for_vars_preserves_disjIdx_validity forbidden_constants trg.rule.body.vars.eraseDupsKeepRight rl v
+    . rw [List.mem_eraseDupsKeepRight]; exact v_mem
+    . apply valid
+      rw [mem_terms_mapped_body_iff]
+      apply Or.inr
+      exists v
+
+theorem PreTrigger.rename_constants_apart_preserves_rule_arity_validity [GetFreshInhabitant sig.C] (trg : PreTrigger sig) (forbidden_constants : List sig.C) :
+    ∀ rl, (h : PreTrigger.skolem_ruleIds_valid rl trg) -> PreTrigger.skolem_rule_arity_valid rl trg h -> PreTrigger.skolem_rule_arity_valid rl (PreTrigger.rename_constants_apart trg forbidden_constants) (PreTrigger.rename_constants_apart_preserves_ruleId_validity trg forbidden_constants rl h) := by
+  intro rl h valid
+  unfold skolem_rule_arity_valid at *
+  intro t t_mem
+  rw [mem_terms_mapped_body_iff] at t_mem
+  cases t_mem with
+  | inl t_mem =>
+    rcases t_mem with ⟨c, c_mem, t_eq⟩
+    simp only [← t_eq]
+    apply GroundTerm.skolem_rule_arity_valid_const
+  | inr t_mem =>
+    rcases t_mem with ⟨v, v_mem, t_eq⟩
+    simp only [← t_eq]
+    apply trg.subs.rename_constants_apart_for_vars_preserves_rule_arity_validity forbidden_constants trg.rule.body.vars.eraseDupsKeepRight rl v
+    . rw [List.mem_eraseDupsKeepRight]; exact v_mem
+    . apply valid
+      rw [mem_terms_mapped_body_iff]
+      apply Or.inr
+      exists v
+
